compiler/backend/proofs/word_simpProofScript.sml
@@ -163,7 +163,7 @@ val dest_Seq_no_inst = prove(``
   every_inst (λi.F) (SND (dest_Seq prog))``,
   ho_match_mp_tac dest_Seq_ind>>rw[dest_Seq_def]>>fs[every_inst_def])
 
-val simp_if_no_inst = store_thm("simp_if_no_inst",``
+val simp_if_no_inst = prove(``
   ∀prog.
   every_inst (λi.F) prog ⇒
   every_inst (λi.F) (simp_if prog)``,
@@ -178,6 +178,20 @@ val simp_if_no_inst = store_thm("simp_if_no_inst",``
   EVERY_CASE_TAC>>fs[SmartSeq_def]>>
   EVERY_CASE_TAC>>rw[]>>rveq>>fs[every_inst_def,dest_If_Eq_Imm_thm]>>
   imp_res_tac dest_Seq_no_inst>> rfs[every_inst_def])
-  dest_If_Eq_Imm_def
+
+val Seq_assoc_no_inst = prove(``
+  ∀p1 p2.
+  every_inst (λi.F) p1 ∧ every_inst (λi.F) p2 ⇒
+  every_inst (λi.F) (Seq_assoc p1 p2)``,
+  ho_match_mp_tac Seq_assoc_ind>>fs[Seq_assoc_def,SmartSeq_def]>>rw[]>>
+  fs[every_inst_def]>>
+  every_case_tac>>fs[])
+
+val compile_exp_no_inst = store_thm("compile_exp_no_inst",``
+  ∀prog.
+  every_inst (λi.F) prog ⇒
+  every_inst (λi.F) (compile_exp prog)``,
+  fs[compile_exp_def]>>
+  metis_tac[simp_if_no_inst,Seq_assoc_no_inst,every_inst_def])
 
 val _ = export_theory();
